src/lib/inst/Kuiper.MatMul.U32.fst
@@ -5,19 +5,25 @@ open Kuiper
 open Kuiper.MatMul
 
 [@@CPrologue "__global__"]
-let kernel_u32 = kernel #u32 R.row_major R.row_major R.row_major
+let kernel_u32
+  : kernel_ty _ _ _ _
+  = kernel #u32 R.row_major R.row_major R.row_major
 
 let matmul_u32 : matmul_ty u32 R.row_major R.row_major R.row_major =
   matmul kernel_u32
 
 [@@CPrologue "__global__"]
-let kernel_u32' = kernel #u32 R.col_major R.col_major R.col_major
+let kernel_u32'
+  : kernel_ty _ _ _ _
+  = kernel #u32 R.col_major R.col_major R.col_major
 
 let matmul_u32' : matmul_ty u32 R.col_major R.col_major R.col_major =
   matmul kernel_u32'
 
 [@@CPrologue "__global__"]
-let kernel_u32'' = kernel #u32 R.col_major R.col_major R.row_major
+let kernel_u32''
+  : kernel_ty _ _ _ _
+  = kernel #u32 R.col_major R.col_major R.row_major
 
 let matmul_u32'' : matmul_ty u32 R.col_major R.col_major R.row_major =
   matmul kernel_u32''
